common/Events.v
@@ -1716,34 +1716,46 @@ Definition meminj_preserves_globals (F V: Type) (ge: Genv.t F V) (f: block -> op
   /\ (forall b gv, Genv.find_var_info ge b = Some gv -> f b = Some(b, 0))
   /\ (forall b1 b2 delta gv, Genv.find_var_info ge b2 = Some gv -> f b1 = Some(b2, delta) -> b2 = b1).
 
-(*
 Lemma external_call_mem_inject:
   forall ef F V (ge: Genv.t F V) vargs m1 t vres m2 f m1' vargs',
   meminj_preserves_globals ge f ->
   external_call ef ge vargs m1 t vres m2 ->
   Mem.inject f m1 m1' ->
   Val.inject_list f vargs vargs' ->
-  exists f', exists vres', exists m2',
-     external_call ef ge vargs' m1' t vres' m2'
-    /\ Val.inject f' vres vres'
-    /\ Mem.inject f' m2 m2'
-    /\ Mem.unchanged_on (loc_unmapped f) m1 m2
-    /\ Mem.unchanged_on (loc_out_of_reach f m1) m1' m2'
-    /\ inject_incr f f'
-    /\ inject_separated f f' m1 m1'.
+  exists t' vres' m2',
+    external_call ef ge vargs' m1' t' vres' m2' /\
+    match_events_query ge cc_inject f t t' /\
+    forall t'',
+      match_traces ge t' t'' ->
+      match_events ge cc_inject f t t'' ->
+      exists f' vres'' m2'',
+        external_call ef ge vargs' m1' t'' vres'' m2'' /\
+        Val.inject f' vres vres'' /\
+        Mem.inject f' m2 m2'' /\
+        Mem.unchanged_on (loc_unmapped f) m1 m2 /\
+        Mem.unchanged_on (loc_out_of_reach f m1) m1' m2'' /\
+        inject_incr f f' /\
+        inject_separated f f' m1 m1'.
 Proof.
-  intros. destruct H as (A & B & C). eapply external_call_mem_inject_gen with (ge1 := ge); eauto.
-  repeat split; intros.
-  + simpl in H3. exploit A; eauto. intros EQ; rewrite EQ in H; inv H. auto.
-  + simpl in H3. exploit A; eauto. intros EQ; rewrite EQ in H; inv H. auto.
-  + simpl in H3. exists b1; split; eauto.
-  + simpl; unfold Genv.block_is_volatile.
-    destruct (Genv.find_var_info ge b1) as [gv1|] eqn:V1.
-    * exploit B; eauto. intros EQ; rewrite EQ in H; inv H. rewrite V1; auto.
-    * destruct (Genv.find_var_info ge b2) as [gv2|] eqn:V2; auto.
-      exploit C; eauto. intros EQ; subst b2. congruence.
+  intros. destruct H as (A & B & C).
+  edestruct external_call_mem_inject_gen
+    as (t' & vres' & m2' & Hstep' & Ht' & Hstep''); eauto.
+  {
+    instantiate (1 := ge).
+    repeat split; intros.
+    + simpl in H3. exploit A; eauto. intros EQ; rewrite EQ in H; inv H. auto.
+    + simpl in H3. exploit A; eauto. intros EQ; rewrite EQ in H; inv H. auto.
+    + simpl in H3. exists b1; split; eauto.
+    + simpl; unfold Genv.block_is_volatile.
+      destruct (Genv.find_var_info ge b1) as [gv1|] eqn:V1.
+      * exploit B; eauto. intros EQ; rewrite EQ in H; inv H. rewrite V1; auto.
+      * destruct (Genv.find_var_info ge b2) as [gv2|] eqn:V2; auto.
+        exploit C; eauto. intros EQ; subst b2. congruence.
+  }
+  exists t', vres', m2'.
+  intuition.
+  edestruct Hstep'' as (vres2'' & m2'' & ? & f' & ?); eauto.
 Qed.
-*)
 
 (** Corollaries of [external_call_determ]. *)
 
